\chapter{Expectation Value of the Swap Operator}
\label{swaperator}
%======================================================================

\begin{align}
\langle \SWA \rangle &=
\bra{\Psi_0\otimes\Psi_0}\SWA \ket{\Psi_0\otimes\Psi_0} \\ &= \nonumber
	\left(\sum_{\alpha'_1,\beta'_1}
		\overline{C}_{\alpha'_1,\beta'_1}\sum_{\alpha'_2,\beta'_2} 
		\overline{C}_{\alpha'_2,\beta'_2}
			\big(\bra{\alpha'_1}\bra{\beta'_1}\big)\otimes\big(\bra{\alpha'_2}\bra{\beta'_2}\big)
			  \right) \times \\ 
	& \hspace{4.2cm}
		\left( \sum_{\alpha_1,\beta_1}C_{\alpha_1,\beta_1}\sum_{\alpha_2,\beta_2} 
			C_{\alpha_2,\beta_2}
			\big(\ket{\alpha_2}\ket{\beta_1}\big)\otimes
			\big(\ket{\alpha_1}\ket{\beta_2}\big) \right) \\
	&=\sum_{\alpha'_1,\beta'_1}\sum_{\alpha_1,\beta_1}
		\overline{C}_{\alpha'_1,\beta'_1}C_{\alpha_1,\beta_1}
		\sum_{\alpha'_2,\beta'_2}\sum_{\alpha_2,\beta_2} 
		\overline{C}_{\alpha'_2,\beta'_2}C_{\alpha_2,\beta_2}
		\inn{\alpha'_1}{\alpha_2}\inn{\beta'_1}{\beta_1}
		\inn{\alpha'_2}{\alpha_1}\inn{\beta'_2}{\beta_2} \\
	&=\sum_{\alpha_1,\beta_1} \sum_{\alpha_2,\beta_2}
		\overline{C}_{\alpha_2,\beta_1}C_{\alpha_1,\beta_1}
		\overline{C}_{\alpha_1,\beta_2}C_{\alpha_2,\beta_2}\\
	&= \sum_{\alpha_1,\alpha_2} \left( \sum_{\beta_1}
		 C_{\alpha_1,\beta_1} \overline{C}_{\alpha_2,\beta_1}\right) 
		 \left( \sum_{\beta_2} C_{\alpha_2,\beta_2} \overline{C}_{\alpha_1,\beta_2}\right)
		\label{mmmm}	
\end{align}
We should pause here to work backwards for a bit.
\begin{align}
	\rho_{\rm A} &= {\rm Tr_B} \ket{\Psi_0} \bra{\Psi_0} \\
	&={\rm Tr_B} \left[ \left(\sum_{\alpha_1,\beta_1} 
		C_{\alpha_1,\beta_1}\ket{\alpha_1}\ket{\beta_1}\right)
		\left(\sum_{\alpha_2,\beta_2} 
		\overline{C}_{\alpha_2,\beta_2}\bra{\alpha_2}\bra{\beta_2}\right) \right] \\
	&=   \sum_{\beta_3} \bra{\beta_3} \left[ \left(\sum_{\alpha_1,\beta_1} 
		C_{\alpha_1,\beta_1}\ket{\alpha_1}\ket{\beta_1}\right)
		\left(\sum_{\alpha_2,\beta_2} 
		\overline{C}_{\alpha_2,\beta_2}\bra{\alpha_2}\bra{\beta_2}\right) \right] \ket{\beta_3} \\
	&=   \sum_{\beta_3}  \left[ \left(\sum_{\alpha_1} 
		C_{\alpha_1,\beta_3}\ket{\alpha_1}\right)
		\left(\sum_{\alpha_2} 
		\overline{C}_{\alpha_2,\beta_3}\bra{\alpha_2}\right) \right] 
\end{align}
If we relabel $\beta_3 \rightarrow \beta_1$ and compute a matrix element:
\begin{align}
	\bra{\alpha_1}\rho_{\rm A} \ket{\alpha_2}
	&=   \bra{\alpha_1}\sum_{\beta_1}  \left[ \left(\sum_{\alpha_1} 
		C_{\alpha_1,\beta_1}\ket{\alpha_1}\right)
		\left(\sum_{\alpha_2} 
		\overline{C}_{\alpha_2,\beta_1}\bra{\alpha_2}\right) \right] \ket{\alpha_2} \\
	&= \sum_{\beta_1} C_{\alpha_1,\beta_1} \overline{C}_{\alpha_2,\beta_1} \label{nnnn},
\end{align}
you may notice that \eqref{nnnn} is one of the expressions found in \eqref{mmmm}.
Now we can continue the calculation of $\langle \SWA \rangle$.
\begin{align}
\langle \SWA \rangle &= \sum_{\alpha_1,\alpha_2} \big( \bra{\alpha_1}\rho_{\rm A} \ket{\alpha_2} 
					\bra{\alpha_2}\rho_{\rm A} \ket{\alpha_1}\big) \\
	&= \sum_{\alpha_1} \big( \bra{\alpha_1}\rho_{\rm A} 
				\underbrace{\sum_{\alpha_2} \ket{\alpha_2}\bra{\alpha_2}}_{\mathds{1}}
				\rho_{\rm A} \ket{\alpha_1}\big) \\
	&= \sum_{\alpha_1} \bra{\alpha_1}\rho_{\rm A}^2  \ket{\alpha_1}
\end{align}
\vspace{-5mm}
\begin{align}
	\hspace{-3.3cm}\boxed{\langle \SWA \rangle= {\rm Tr (\rho_A^2)}} \hspace{1cm}
\end{align}

